Foundation/Modal/Kripke2/AxiomDot3.lean
@@ -1,0 +1,46 @@
+import Foundation.Modal.Kripke2.Basic
+
+namespace LO.Modal
+
+open Formula.Kripke
+
+namespace Kripke
+
+variable {F : Kripke.Frame}
+
+lemma connected_of_validate_dot3 (hCon : Connected F) : F ⊧ (Axioms.Dot3 (.atom 0) (.atom 1)) := by
+  rintro V x;
+  apply Satisfies.or_def.mpr;
+  suffices
+    (∀ y, x ≺ y → (∀ z, y ≺ z → V z 0) → V y 1) ∨
+    (∀ y, x ≺ y → (∀ z, y ≺ z → V z 1) → V y 0)
+    by simpa [Semantics.Realize, Satisfies];
+  by_contra hC;
+  push_neg at hC;
+  obtain ⟨⟨y, Rxy, hp, hnq⟩, ⟨z, Rxz, hq, hnp⟩⟩ := hC;
+  cases hCon ⟨Rxy, Rxz⟩ with
+  | inl Ryz => have := hp z Ryz; contradiction;
+  | inr Rzy => have := hq y Rzy; contradiction;
+
+lemma validate_dot3_of_connected : F ⊧ (Axioms.Dot3 (.atom 0) (.atom 1)) → Connected F := by
+  contrapose;
+  intro hCon;
+  obtain ⟨x, y, Rxy, z, Ryz, nRyz, nRzy⟩ := by simpa [Connected] using hCon;
+  apply ValidOnFrame.not_of_exists_valuation_world;
+  use (λ w a => match a with | 0 => y ≺ w | 1 => z ≺ w | _ => False), x;
+  suffices ∃ y', x ≺ y' ∧ (∀ z', y' ≺ z' → y ≺ z') ∧ ¬z ≺ y' ∧ (∃ z', x ≺ z' ∧ (∀ y, z' ≺ y → z ≺ y) ∧ ¬y ≺ z') by
+    simpa [Semantics.Realize, Satisfies];
+  refine ⟨y, Rxy, by tauto, nRzy, z, Ryz, by tauto, nRyz⟩;
+
+abbrev ConnectedFrameClass : FrameClass := { F | Connected F }
+
+instance ConnectedFrameClass.DefinedByDot3 : ConnectedFrameClass.DefinedBy {Axioms.Dot3 (.atom 0) (.atom 1)} := ⟨by
+  intro F;
+  constructor;
+  . simpa using connected_of_validate_dot3;
+  . simpa using validate_dot3_of_connected;
+⟩
+
+end Kripke
+
+end LO.Modal
