Foundation/Modal/Kripke2/AxiomGeach.lean
@@ -1,0 +1,211 @@
+import Foundation.Vorspiel.BinaryRelations
+import Foundation.Modal.Kripke2.Completeness
+import Foundation.Modal.Kripke2.Basic
+import Foundation.Modal.Hilbert2.Geach
+
+def MultiGeachean (ts : Set GeachConfluent.Taple) (R : Rel α α) := ∀ t ∈ ts, GeachConfluent t R
+
+
+namespace LO.Modal
+
+namespace Kripke
+
+abbrev GeachConfluentFrameClass (t : GeachConfluent.Taple) : FrameClass := { F | (GeachConfluent t) F.Rel }
+
+instance GeachConfluentFrameClass.nonempty : (GeachConfluentFrameClass t).Nonempty := by
+  use ⟨Unit, λ _ _ => True⟩;
+  intros x _ _ _; use x;
+  constructor <;> { apply Rel.iterate.true_any; tauto; }
+
+
+abbrev MultiGeacheanConfluentFrameClass (ts : Set GeachConfluent.Taple) : FrameClass := { F | (MultiGeachean ts) F.Rel }
+
+instance MultiGeacheanConfluentFrameClass.nonempty : (MultiGeacheanConfluentFrameClass ts).Nonempty := by
+  use ⟨Unit, λ _ _ => True⟩;
+  intros t ht x y z h;
+  use x;
+  constructor <;> { apply Rel.iterate.true_any; tauto; }
+
+open Formula.Kripke
+
+instance MultiGeachConfluentFrameClass.isDefinedBy (ts) : (MultiGeacheanConfluentFrameClass ts).DefinedBy (ts.image (λ t => Axioms.Geach t (.atom 0))) := by
+  unfold MultiGeacheanConfluentFrameClass MultiGeachean Axioms.Geach;
+  constructor;
+  intro F;
+  constructor;
+  . rintro hF φ ⟨t, ⟨ht, rfl⟩⟩ V x h;
+    obtain ⟨y, Rxy, hbp⟩ := Satisfies.multidia_def.mp h;
+    apply Satisfies.multibox_def.mpr;
+    intro z Rxz;
+    apply Satisfies.multidia_def.mpr;
+    obtain ⟨u, Ryu, Rzu⟩ := hF t ht ⟨Rxy, Rxz⟩;
+    use u;
+    constructor;
+    . assumption;
+    . exact (Satisfies.multibox_def.mp hbp) Ryu;
+  . rintro h t ht x y z ⟨Rxy, Rxz⟩;
+    let V : Kripke.Valuation F := λ v _ => y ≺^[t.m] v;
+    have : Satisfies ⟨F, V⟩ x (◇^[t.i](□^[t.m](.atom 0))) := by
+      apply Satisfies.multidia_def.mpr;
+      use y;
+      constructor;
+      . assumption;
+      . apply Satisfies.multibox_def.mpr;
+        aesop;
+    have : Satisfies ⟨F, V⟩ x (□^[t.j](◇^[t.n]Formula.atom 0)) := h (Axioms.Geach t (.atom 0)) (by tauto) V x this;
+    have : Satisfies ⟨F, V⟩ z (◇^[t.n]Formula.atom 0) := Satisfies.multibox_def.mp this Rxz;
+    obtain ⟨u, Rzu, Ryu⟩ := Satisfies.multidia_def.mp this;
+    exact ⟨u, Ryu, Rzu⟩;
+
+instance GeachConfluentFrameClass.isDefinedBy (t) : (GeachConfluentFrameClass t).DefinedByFormula (Axioms.Geach t (.atom 0)) := by
+  have := MultiGeachConfluentFrameClass.isDefinedBy {t};
+  simp at this;
+  constructor;
+  intro F;
+  constructor;
+  . rintro hF _ ⟨_, rfl⟩;
+    apply this.defines F |>.mp;
+    . simp_all [MultiGeachean];
+    . simp;
+  . intro h;
+    apply this.defines F |>.mpr <;> tauto;
+
+
+section
+
+abbrev ReflexiveFrameClass   : FrameClass := { F | Reflexive F.Rel }
+abbrev SerialFrameClass      : FrameClass := { F | Serial F.Rel }
+abbrev SymmetricFrameClass   : FrameClass := { F | Symmetric F.Rel }
+abbrev TransitiveFrameClass  : FrameClass := { F | Transitive F.Rel }
+abbrev EuclideanFrameClass   : FrameClass := { F | Euclidean F.Rel }
+abbrev ConfluentFrameClass   : FrameClass := { F | Confluent F.Rel }
+abbrev FunctionalFrameClass  : FrameClass := { F | Functional F.Rel }
+abbrev CoreflexiveFrameClass : FrameClass := { F | Coreflexive F.Rel }
+abbrev DenseFrameClass       : FrameClass := { F | Dense F.Rel }
+
+abbrev ReflexiveEuclideanFrameClass : FrameClass := { F | Reflexive F.Rel ∧ Euclidean F.Rel }
+abbrev ReflexiveSymmetricFrameClass : FrameClass := { F | Reflexive F ∧ Symmetric F }
+abbrev ReflexiveTransitiveFrameClass : FrameClass := { F | Reflexive F ∧ Transitive F }
+abbrev ReflexiveTransitiveConfluentFrameClass : FrameClass := { F | Reflexive F ∧ Transitive F ∧ Confluent F }
+abbrev ReflexiveTransitiveSymmetricFrameClass : FrameClass := { F | Reflexive F ∧ Transitive F ∧ Symmetric F }
+abbrev SerialTransitiveEuclideanFrameClass : FrameClass := { F | Serial F ∧ Transitive F ∧ Euclidean F }
+abbrev TransitiveEuclideanFrameClass : FrameClass := { F | Transitive F ∧ Euclidean F }
+abbrev SymmetricTransitiveFrameClass : FrameClass := { F | Symmetric F ∧ Transitive F }
+abbrev SymmetricEuclideanFrameClass : FrameClass := { F | Symmetric F ∧ Euclidean F }
+abbrev SerialSymmetricFrameClass : FrameClass := { F | Serial F ∧ Symmetric F }
+abbrev SerialTransitiveFrameClass : FrameClass := { F | Serial F ∧ Transitive F }
+abbrev SerialEuclideanFrameClass : FrameClass := { F | Serial F ∧ Euclidean F }
+
+end
+
+
+instance ReflexiveFrameClass.DefinedByAxiomT : ReflexiveFrameClass.DefinedByFormula (Axioms.T (.atom 0)) := by
+  rw [
+    (show ReflexiveFrameClass = GeachConfluentFrameClass ⟨0, 0, 1, 0⟩ by
+      ext;
+      simp only [Set.mem_setOf_eq];
+      exact GeachConfluent.reflexive_def
+    ),
+    (show Axioms.T (.atom 0) = (Axioms.Geach ⟨0, 0, 1, 0⟩ (Formula.atom 0)) by rfl)
+  ];
+  exact GeachConfluentFrameClass.isDefinedBy _;
+
+
+instance SerialFrameClass.DefinedByAxiomD : SerialFrameClass.DefinedByFormula (Axioms.D (.atom 0)) := by
+  rw [
+    (show SerialFrameClass = GeachConfluentFrameClass ⟨0, 0, 1, 1⟩ by
+      ext;
+      simp only [Set.mem_setOf_eq];
+      exact GeachConfluent.serial_def;
+    ),
+    (show Axioms.D (.atom 0) = (Axioms.Geach ⟨0, 0, 1, 1⟩ (Formula.atom 0)) by rfl)
+  ];
+  exact GeachConfluentFrameClass.isDefinedBy _;
+
+
+instance SymmetricFrameClass.DefinedByAxiomB : SymmetricFrameClass.DefinedByFormula (Axioms.B (.atom 0)) := by
+  rw [
+    (show SymmetricFrameClass = GeachConfluentFrameClass ⟨0, 1, 0, 1⟩ by
+      ext;
+      simp only [Set.mem_setOf_eq];
+      exact GeachConfluent.symmetric_def;
+    ),
+    (show Axioms.B (.atom 0) = (Axioms.Geach ⟨0, 1, 0, 1⟩ (Formula.atom 0)) by rfl)
+  ];
+  exact GeachConfluentFrameClass.isDefinedBy _;
+
+
+instance TransitiveFrameClass.DefinedByAxiomFour : TransitiveFrameClass.DefinedByFormula (Axioms.Four (.atom 0)) := by
+  rw [
+    (show TransitiveFrameClass = GeachConfluentFrameClass ⟨0, 2, 1, 0⟩ by
+      ext;
+      simp only [Set.mem_setOf_eq];
+      exact GeachConfluent.transitive_def;
+    ),
+    (show Axioms.Four (.atom 0) = (Axioms.Geach ⟨0, 2, 1, 0⟩ (Formula.atom 0)) by rfl)
+  ];
+  exact GeachConfluentFrameClass.isDefinedBy _;
+
+
+instance EuclideanFrameClass.DefinedByAxiomFive : EuclideanFrameClass.DefinedByFormula (Axioms.Five (.atom 0)) := by
+  rw [
+    (show EuclideanFrameClass = GeachConfluentFrameClass ⟨1, 1, 0, 1⟩ by
+      ext;
+      simp only [Set.mem_setOf_eq];
+      exact GeachConfluent.euclidean_def;
+    ),
+    (show Axioms.Five (.atom 0) = (Axioms.Geach ⟨1, 1, 0, 1⟩ (Formula.atom 0)) by rfl)
+  ];
+  exact GeachConfluentFrameClass.isDefinedBy _;
+
+
+instance ConfluentFrameClass.DefinedByAxiomDot2 : ConfluentFrameClass.DefinedByFormula (Axioms.Dot2 (.atom 0)) := by
+  rw [
+    (show ConfluentFrameClass = GeachConfluentFrameClass ⟨1, 1, 1, 1⟩ by
+      ext;
+      simp only [Set.mem_setOf_eq];
+      exact GeachConfluent.confluent_def;
+    ),
+    (show Axioms.Dot2 (.atom 0) = (Axioms.Geach ⟨1, 1, 1, 1⟩ (Formula.atom 0)) by rfl)
+  ];
+  exact GeachConfluentFrameClass.isDefinedBy _;
+
+
+instance FunctionalFrameClass.DefinedByAxiomCD : FunctionalFrameClass.DefinedByFormula (Axioms.CD (.atom 0)) := by
+  rw [
+    (show FunctionalFrameClass = GeachConfluentFrameClass ⟨1, 1, 0, 0⟩ by
+      ext;
+      simp only [Set.mem_setOf_eq];
+      exact GeachConfluent.functional_def;
+    ),
+    (show Axioms.CD (.atom 0) = (Axioms.Geach ⟨1, 1, 0, 0⟩ (Formula.atom 0)) by rfl)
+  ];
+  exact GeachConfluentFrameClass.isDefinedBy _;
+
+
+instance CoreflexiveFrameClass.DefinedByAxiomTc : CoreflexiveFrameClass.DefinedByFormula (Axioms.Tc (.atom 0)) := by
+  rw [
+    (show CoreflexiveFrameClass = GeachConfluentFrameClass ⟨0, 1, 0, 0⟩ by
+      ext;
+      simp only [Set.mem_setOf_eq];
+      exact GeachConfluent.extensive_def;
+    ),
+    (show Axioms.Tc (.atom 0) = (Axioms.Geach ⟨0, 1, 0, 0⟩ (Formula.atom 0)) by rfl)
+  ];
+  exact GeachConfluentFrameClass.isDefinedBy _;
+
+
+instance DenseFrameClass.DefinedByAxiomC4 : DenseFrameClass.DefinedByFormula (Axioms.C4 (.atom 0)) := by
+  rw [
+    (show DenseFrameClass = GeachConfluentFrameClass ⟨0, 1, 2, 0⟩ by
+      ext;
+      simp only [Set.mem_setOf_eq];
+      exact GeachConfluent.dense_def;
+    ),
+    (show Axioms.C4 (.atom 0) = (Axioms.Geach ⟨0, 1, 2, 0⟩ (Formula.atom 0)) by rfl)
+  ];
+  exact GeachConfluentFrameClass.isDefinedBy _;
+
+end Kripke
+
+end LO.Modal
