Foundation/Modal/Kripke2/FiniteFrame.lean
@@ -1,0 +1,110 @@
+import Foundation.Modal.Kripke2.Basic
+
+namespace LO.Modal
+
+namespace Kripke
+
+structure FiniteFrame extends Frame where
+  [world_finite : Finite toFrame.World]
+
+instance {F : FiniteFrame} : Finite F.World := F.world_finite
+
+
+def Frame.toFinite (F : Frame) [Finite F.World] : FiniteFrame where
+  toFrame := F
+
+
+abbrev FiniteFrameClass := Set FiniteFrame
+
+def FrameClass.restrictFinite (C : FrameClass) : FiniteFrameClass := { F : FiniteFrame | F.toFrame ∈ C }
+
+def FiniteFrameClass.toFrameClass (C : FiniteFrameClass) : FrameClass := C.image (·.toFrame)
+
+instance : Coe (FiniteFrameClass) (FrameClass) := ⟨FiniteFrameClass.toFrameClass⟩
+
+
+abbrev reflexivePointFrame : FiniteFrame where
+  World := Unit
+  Rel := fun _ _ => True
+
+abbrev irreflexivePointFrame : FiniteFrame where
+  World := Unit
+  Rel := fun _ _ => False
+
+abbrev AllFiniteFrameClass : FiniteFrameClass := Set.univ
+
+end Kripke
+
+
+namespace Formula.Kripke
+
+def ValidOnFiniteFrame (F : Kripke.FiniteFrame) (φ : Formula ℕ) := F.toFrame ⊧ φ
+
+namespace ValidOnFiniteFrame
+
+instance semantics : Semantics (Formula ℕ) (Kripke.FiniteFrame) := ⟨fun F ↦ Formula.Kripke.ValidOnFiniteFrame F⟩
+
+variable {F : Kripke.FiniteFrame}
+
+@[simp] protected lemma models_iff : F ⊧ φ ↔ Kripke.ValidOnFiniteFrame F φ := iff_of_eq rfl
+
+lemma models_set_iff : F ⊧* Φ ↔ ∀ φ ∈ Φ, F ⊧ φ := by simp [Semantics.realizeSet_iff];
+
+protected lemma top_def : F ⊧ ⊤ := by simp [ValidOnFiniteFrame];
+
+protected lemma bot_def : ¬F ⊧ ⊥ := by simp [ValidOnFiniteFrame];
+
+instance : Semantics.Top (Kripke.FiniteFrame) where
+  realize_top _ := ValidOnFrame.top_def;
+
+instance : Semantics.Bot (Kripke.FiniteFrame) where
+  realize_bot _ := ValidOnFrame.bot_def
+
+lemma iff_not_exists_valuation : (¬F ⊧ φ) ↔ (∃ V : Kripke.Valuation F.toFrame, ¬(⟨F.toFrame, V⟩ : Kripke.Model) ⊧ φ) := by
+  exact ValidOnFrame.iff_not_exists_valuation;
+
+alias ⟨exists_valuation_of_not, not_of_exists_valuation⟩ := iff_not_exists_valuation
+
+lemma iff_not_exists_valuation_world : (¬F ⊧ φ) ↔ (∃ V : Kripke.Valuation F.toFrame, ∃ x : (⟨F.toFrame, V⟩ : Kripke.Model).World, ¬Satisfies _ x φ) := by
+  exact ValidOnFrame.iff_not_exists_valuation_world;
+
+alias ⟨exists_valuation_world_of_not, not_of_exists_valuation_world⟩ := iff_not_exists_valuation_world
+
+end ValidOnFiniteFrame
+
+
+def ValidOnFiniteFrameClass (C : Kripke.FiniteFrameClass) (φ : Formula ℕ) := C.toFrameClass ⊧ φ
+
+namespace ValidOnFiniteFrameClass
+
+protected instance semantics : Semantics (Formula ℕ) (Kripke.FiniteFrameClass) := ⟨fun C ↦ Kripke.ValidOnFrameClass C⟩
+
+variable {C : Kripke.FiniteFrameClass}
+
+@[simp] protected lemma models_iff : C ⊧ φ ↔ Formula.Kripke.ValidOnFrameClass C φ := iff_of_eq rfl
+
+lemma iff_not_exists_frame : (¬C ⊧ φ) ↔ (∃ F ∈ C, ¬F ⊧ φ) := by
+  convert ValidOnFrameClass.iff_not_exists_frame;
+  simp [Kripke.FiniteFrameClass.toFrameClass, ValidOnFiniteFrame ];
+
+alias ⟨exists_frame_of_not, not_of_exists_frame⟩ := iff_not_exists_frame
+
+end ValidOnFiniteFrameClass
+
+end Formula.Kripke
+
+
+namespace Kripke
+
+class FiniteFrameClass.DefinedBy (C : Kripke.FiniteFrameClass) (Γ : Set (Formula ℕ)) where
+  defines : ∀ F, F ∈ C ↔ (∀ φ ∈ Γ, F ⊧ φ)
+
+class FiniteFrameClass.FiniteDefinedBy (C Γ) extends FiniteFrameClass.DefinedBy C Γ where
+  finite : Set.Finite Γ
+
+class FiniteFrameClass.IsNonempty (C : Kripke.FiniteFrameClass) where
+  nonempty : Nonempty C
+
+end Kripke
+
+end LO.Modal
