Foundation/Modal/Kripke2/Hilbert/K.lean
@@ -4,11 +4,12 @@ import Foundation.Modal.Kripke2.Completeness
 
 namespace LO.Modal
 
-instance : Kripke.AllFrameClass.DefinedBy (Hilbert.K.axioms) := ⟨by
+instance FrameClass.DefinedBy : Kripke.AllFrameClass.DefinedBy (Hilbert.K.axioms) := ⟨by
   suffices ∀ F, ∀ φ ∈ Hilbert.K.axioms, Formula.Kripke.ValidOnFrame F φ by simpa;
   rintro F _ ⟨ψ, ⟨_, rfl⟩, ⟨s, rfl⟩⟩;
   apply Formula.Kripke.ValidOnFrame.axiomK;
 ⟩
+
 
 namespace Hilbert.K
 
@@ -17,5 +18,6 @@ instance : System.Consistent (Hilbert.K) := Kripke.Hilbert.instConsistent (C := 
 instance : Complete (Hilbert.K) (Kripke.AllFrameClass) := Kripke.instCompleteOfCanonical trivial
 
 end Hilbert.K
+
 
 end LO.Modal
