Foundation/Modal/Kripke2/NNFormula.lean
@@ -1,0 +1,266 @@
+import Foundation.Modal.NNFormula
+import Foundation.Modal.Kripke2.Basic
+
+namespace LO.Modal
+
+open System
+
+variable {φ ψ : NNFormula ℕ}
+
+namespace NNFormula.Kripke
+
+def Satisfies (M : Kripke.Model) (x : M.World) : NNFormula ℕ → Prop
+  | atom a  =>  M x a
+  | natom a => ¬M x a
+  | ⊤       => True
+  | ⊥       => False
+  | φ ⋎ ψ   => Satisfies M x φ ∨ Satisfies M x ψ
+  | φ ⋏ ψ   => Satisfies M x φ ∧ Satisfies M x ψ
+  | □φ      => ∀ y, x ≺ y → Satisfies M y φ
+  | ◇φ      => ∃ y, x ≺ y ∧ (Satisfies M y φ)
+
+namespace Satisfies
+
+variable {M : Kripke.Model} {x : M.World}
+
+protected instance semantics : Semantics (NNFormula ℕ) (M.World) := ⟨λ x ↦ Satisfies M x⟩
+
+protected lemma iff_models : x ⊧ φ ↔ Satisfies M x φ := iff_of_eq rfl
+
+@[simp]
+protected lemma atom_def (a : ℕ) : x ⊧ (atom a) ↔ M x a := by simp [Satisfies.iff_models, Satisfies];
+
+@[simp]
+protected lemma natom_def (a : ℕ) : x ⊧ (natom a) ↔ ¬M x a := by simp [Satisfies.iff_models, Satisfies];
+
+protected lemma top_def : x ⊧ ⊤ := by simp [Satisfies.iff_models, Satisfies];
+
+protected lemma bot_def : ¬x ⊧ ⊥ := by simp [Satisfies.iff_models, Satisfies];
+
+protected lemma or_def : x ⊧ φ ⋎ ψ ↔ x ⊧ φ ∨ x ⊧ ψ := by simp [Satisfies.iff_models, Satisfies];
+
+protected lemma and_def : x ⊧ φ ⋏ ψ ↔ x ⊧ φ ∧ x ⊧ ψ := by simp [Satisfies.iff_models, Satisfies];
+
+protected lemma box_def : x ⊧ □φ ↔ ∀ y, x ≺ y → y ⊧ φ := by simp [Satisfies.iff_models, Satisfies];
+
+protected lemma dia_def : x ⊧ ◇φ ↔ ∃ y, x ≺ y ∧ y ⊧ φ := by simp [Satisfies.iff_models, Satisfies];
+
+protected lemma neg_def : x ⊧ ∼φ ↔ ¬x ⊧ φ := by
+  induction φ using NNFormula.rec' generalizing x with
+  | hOr φ ψ ihφ ihψ =>
+    simp only [DeMorgan.or, Satisfies.or_def, not_or];
+    constructor;
+    . rintro ⟨h₁, h₂⟩;
+      exact ⟨ihφ.mp h₁, ihψ.mp h₂⟩;
+    . rintro ⟨h₁, h₂⟩;
+      exact ⟨ihφ.mpr h₁, ihψ.mpr h₂⟩;
+  | hAnd φ ψ ihφ ihψ =>
+    simp only [DeMorgan.and, Satisfies.and_def, not_and_or];
+    constructor;
+    . rintro (h₁ | h₂);
+      . left; exact ihφ.mp h₁;
+      . right; exact ihψ.mp h₂;
+    . rintro (h₁ | h₂);
+      . left; exact ihφ.mpr h₁;
+      . right; exact ihψ.mpr h₂;
+  | hBox φ ihφ =>
+    simp only [ModalDeMorgan.box, Satisfies.box_def];
+    push_neg;
+    constructor;
+    . intro h;
+      obtain ⟨y, Rxy, hy⟩ := h;
+      use y;
+      constructor;
+      . exact Rxy;
+      . apply ihφ.mp;
+        exact hy;
+    . rintro ⟨y, Rxy, h⟩;
+      use y;
+      constructor;
+      . exact Rxy;
+      . apply ihφ.mpr;
+        exact h;
+  | hDia φ ihφ =>
+    simp only [ModalDeMorgan.dia, Satisfies.dia_def, not_exists, not_and];
+    constructor;
+    . intro h y Rxy;
+      apply ihφ.mp;
+      exact h y Rxy;
+    . intro h y Rxy;
+      apply ihφ.mpr;
+      exact h y Rxy;
+  | _ => simp [Satisfies.iff_models, Satisfies];
+
+protected lemma imp_def : x ⊧ φ ➝ ψ ↔ x ⊧ φ → x ⊧ ψ := by
+  simp [←NNFormula.imp_eq, NNFormula.imp, Satisfies.or_def, Satisfies.neg_def];
+  tauto;
+
+protected instance : Semantics.Tarski (M.World) where
+  realize_top := λ _ => Satisfies.top_def
+  realize_bot := λ _ => Satisfies.bot_def
+  realize_or  := Satisfies.or_def
+  realize_and := Satisfies.and_def
+  realize_imp := Satisfies.imp_def
+  realize_not := Satisfies.neg_def
+
+end Satisfies
+
+
+def ValidOnModel (M : Kripke.Model) := λ φ => ∀ x, Satisfies M x φ
+
+namespace ValidOnModel
+
+instance semantics : Semantics (NNFormula ℕ) (Kripke.Model) := ⟨λ M ↦ ValidOnModel M⟩
+
+@[simp] protected lemma iff_models : M ⊧ φ ↔ ValidOnModel M φ := iff_of_eq rfl
+
+end ValidOnModel
+
+
+def ValidOnFrame (F : Kripke.Frame) := λ φ => ∀ V, (⟨F, V⟩ : Kripke.Model) ⊧ φ
+
+namespace ValidOnFrame
+
+instance semantics : Semantics (NNFormula ℕ) (Kripke.Frame) := ⟨λ F ↦ ValidOnFrame F⟩
+
+@[simp] protected lemma iff_models : F ⊧ φ ↔ ValidOnFrame F φ := iff_of_eq rfl
+
+end ValidOnFrame
+
+
+def ValidOnFrameClass (C : Kripke.FrameClass) := λ φ => ∀ {F}, F ∈ C → ValidOnFrame F φ
+
+namespace ValidOnFrameClass
+
+instance semantics : Semantics (NNFormula ℕ) (Kripke.FrameClass) := ⟨λ C ↦ ValidOnFrameClass C⟩
+
+@[simp] protected lemma iff_models : C ⊧ φ ↔ ValidOnFrameClass C φ := iff_of_eq rfl
+
+end ValidOnFrameClass
+
+end NNFormula.Kripke
+
+
+namespace NNFormula.Kripke
+
+variable {φ : NNFormula ℕ}
+
+lemma Satisfies.toFormula : NNFormula.Kripke.Satisfies M x φ ↔ Formula.Kripke.Satisfies M x φ.toFormula := by
+  induction φ using NNFormula.rec' generalizing x with
+  | hOr φ ψ ihφ ihψ =>
+    constructor;
+    . rintro (hφ | hψ);
+      . apply Formula.Kripke.Satisfies.or_def.mpr;
+        left;
+        exact ihφ.mp hφ;
+      . apply Formula.Kripke.Satisfies.or_def.mpr;
+        right;
+        exact ihψ.mp hψ;
+    . rintro h;
+      rcases Formula.Kripke.Satisfies.or_def.mp h with (hφ | hψ);
+      . left; exact ihφ.mpr hφ;
+      . right; exact ihψ.mpr hψ;
+  | hAnd φ ψ ihφ ihψ =>
+    constructor;
+    . rintro ⟨hφ, hψ⟩;
+      apply Formula.Kripke.Satisfies.and_def.mpr;
+      constructor;
+      . exact ihφ.mp hφ;
+      . exact ihψ.mp hψ;
+    . rintro h;
+      replace ⟨hφ, hψ⟩ := Formula.Kripke.Satisfies.and_def.mp h;
+      constructor;
+      . apply ihφ.mpr hφ;
+      . apply ihψ.mpr hψ;
+  | hBox φ ihφ =>
+    constructor;
+    . intro h y Rxy;
+      apply ihφ.mp;
+      exact h y Rxy;
+    . intro h y Rxy;
+      apply ihφ.mpr;
+      exact h y Rxy;
+  | hDia φ ihφ =>
+    constructor;
+    . rintro ⟨y, Rxy, hy⟩;
+      apply Formula.Kripke.Satisfies.dia_def.mpr;
+      use y;
+      constructor;
+      . exact Rxy;
+      . apply ihφ.mp;
+        exact hy;
+    . rintro h;
+      obtain ⟨y, Rxy, hy⟩ := Formula.Kripke.Satisfies.dia_def.mp h;
+      use y;
+      constructor;
+      . exact Rxy;
+      . apply ihφ.mpr;
+        exact hy;
+  | _ => simp [NNFormula.Kripke.Satisfies, Formula.Kripke.Satisfies];
+
+lemma ValidOnModel.toFormula : NNFormula.Kripke.ValidOnModel M φ ↔ Formula.Kripke.ValidOnModel M φ.toFormula := by
+  simp only [NNFormula.Kripke.ValidOnModel, Formula.Kripke.ValidOnModel, Satisfies.toFormula];
+  exact ⟨λ h x => h x, λ h x => h x⟩;
+
+lemma ValidOnFrame.toFormula : NNFormula.Kripke.ValidOnFrame F φ ↔ Formula.Kripke.ValidOnFrame F φ.toFormula := ⟨
+  λ h V => ValidOnModel.toFormula.mp (h V),
+  λ h V => ValidOnModel.toFormula.mpr (h V)
+⟩
+
+lemma ValidOnFrameClass.toFormula : NNFormula.Kripke.ValidOnFrameClass C φ ↔ Formula.Kripke.ValidOnFrameClass C φ.toFormula := ⟨
+  λ h _ hF => ValidOnFrame.toFormula.mp (h hF),
+  λ h _ hF => ValidOnFrame.toFormula.mpr (h hF)
+⟩
+
+end NNFormula.Kripke
+
+
+namespace Formula.Kripke
+
+variable {φ : Formula ℕ}
+
+lemma Satisfies.toNNFormula : Formula.Kripke.Satisfies M x φ ↔ NNFormula.Kripke.Satisfies M x φ.toNNFormula := by
+  induction φ using Formula.rec' generalizing x with
+  | hbox φ ihφ =>
+    constructor;
+    . intro h y Rxy;
+      apply ihφ.mp;
+      exact h y Rxy;
+    . intro h y Rxy;
+      apply ihφ.mpr;
+      exact h y Rxy;
+  | himp φ ψ ihφ ihψ =>
+    constructor;
+    . rintro h;
+      apply NNFormula.Kripke.Satisfies.imp_def.mpr;
+      intro hφ;
+      apply ihψ.mp;
+      apply h;
+      apply ihφ.mpr;
+      exact hφ;
+    . intro h hφ;
+      apply ihψ.mpr;
+      apply NNFormula.Kripke.Satisfies.imp_def.mp h;
+      apply ihφ.mp;
+      exact hφ;
+  | _ => simp [Formula.Kripke.Satisfies, NNFormula.Kripke.Satisfies];
+
+lemma ValidOnModel.toNNFormula : Formula.Kripke.ValidOnModel M φ ↔ NNFormula.Kripke.ValidOnModel M φ.toNNFormula := ⟨
+  fun h x => Satisfies.toNNFormula.mp (h x),
+  fun h x => Satisfies.toNNFormula.mpr (h x)
+⟩
+
+lemma ValidOnFrame.toNNFormula : Formula.Kripke.ValidOnFrame F φ ↔ NNFormula.Kripke.ValidOnFrame F φ.toNNFormula := ⟨
+  fun h V => ValidOnModel.toNNFormula.mp (h V),
+  fun h V => ValidOnModel.toNNFormula.mpr (h V)
+⟩
+
+lemma ValidOnFrameClass.toNNFormula : Formula.Kripke.ValidOnFrameClass C φ ↔ NNFormula.Kripke.ValidOnFrameClass C φ.toNNFormula := ⟨
+  fun h _ hF => ValidOnFrame.toNNFormula.mp (h hF),
+  fun h _ hF => ValidOnFrame.toNNFormula.mpr (h hF)
+⟩
+
+end Formula.Kripke
+
+
+end LO.Modal
