Foundation/Modal/Kripke2/Universal.lean
@@ -1,0 +1,21 @@
+import Foundation.Modal.Kripke2.AxiomGeach
+import Foundation.Modal.Kripke2.Preservation
+
+namespace LO.Modal
+
+namespace Kripke
+
+abbrev UniversalFrameClass : FrameClass := { F | Universal F }
+
+lemma iff_Universal_ReflexiveEuclidean_validOnFrameClass : UniversalFrameClass ⊧ φ ↔ ReflexiveEuclideanFrameClass ⊧ φ := by
+  constructor;
+  . intro h F hF V r;
+    let M : Model := ⟨F, V⟩;
+    apply Model.PointGenerated.modal_equivalent_at_root  (M := ⟨F, V⟩) (by apply trans_of_refl_eucl hF.1 hF.2) r |>.mp;
+    apply @h (F↾r).toFrame (Frame.PointGenerated.rel_universal hF.1 hF.2) (M↾r).Val;
+  . rintro h F F_univ;
+    exact @h F (⟨refl_of_universal F_univ, eucl_of_universal F_univ⟩);
+
+end Kripke
+
+end LO.Modal
